Stuck at simultaneous ver of the refl property

typing_properties.v
@@ -65,3 +65,73 @@ Proof.
     by asimpl.
     by asimpl.
 Qed.
+
+Lemma equiv_renaming Γ A B (h : Γ ⊢ A ≡ B) :
+  forall ξ Δ, lookup_good_renaming ξ Γ Δ -> ⊢ Δ -> Δ ⊢ A⟨ξ⟩ ≡ B⟨ξ⟩.
+Proof.
+  elim : A B / h; hauto q:on ctrs:WtEquiv use:wt_renaming_mutual.
+Qed.
+
+Definition lookup_good_morphing ρ0 ρ1 Γ Δ :=
+  forall n A, lookup n Γ A -> Δ ⊢ ρ0 n ▻ ρ1 n ∈ A[ρ0].
+
+Lemma lookup_good_renaming_shift A Δ:
+  lookup_good_renaming ↑ Δ (A :: Δ).
+Proof. rewrite /lookup_good_renaming => >. apply there. Qed.
+
+Lemma subst_ren_factor A ρ ξ :  A[ρ >> ren_tm ξ ] = A[ρ]⟨ξ⟩.
+Proof. by asimpl. Qed.
+
+Lemma good_morphing_up ρ0 ρ1 k Γ Δ A
+  (h : lookup_good_morphing ρ0 ρ1 Γ Δ) :
+  Δ ⊢ A[ρ0] ▻ A[ρ1] ∈ Univ k ->
+  lookup_good_morphing (up_tm_tm ρ0) (up_tm_tm ρ1) (A :: Γ) (A [ρ0] :: Δ).
+Proof.
+  rewrite /lookup_good_morphing => h1.
+  inversion 1=>*; subst.
+  - apply WR_Var => /=.
+    + eauto with wt.
+    + asimpl. apply : here'. by asimpl.
+  - asimpl. rewrite !subst_ren_factor.
+    eapply wt_renaming_mutual. hauto l:on unfold:lookup_good_morphing.
+    apply lookup_good_renaming_shift.
+    eauto with wt.
+Qed.
+
+Lemma wt_morphing_mutual :
+  (forall Γ a b A, Γ ⊢ a ▻ b ∈ A -> forall ρ0 ρ1 Δ,
+        lookup_good_morphing ρ0 ρ1 Γ Δ -> Wf Δ -> Δ ⊢ a[ρ0] ▻ a[ρ1] ∈ A[ρ0] ) /\
+  (forall Γ a b A, Γ ⊢ a ▻+ b ∈ A -> forall ρ0 ρ1 Δ,
+        lookup_good_morphing ρ0 ρ1 Γ Δ -> Wf Δ -> Δ ⊢ a[ρ0] ▻+ a[ρ1] ∈ A[ρ0] ) /\
+  (forall Γ, ⊢ Γ -> forall ρ0 ρ1 Δ, lookup_good_morphing ρ0 ρ1 Γ Δ -> Wf Δ -> lookup_good_morphing ρ0 ρ0 Γ Δ).
+Proof.
+  apply wt_mutual_ind; eauto with wt.
+  8 : {
+    hauto q:on inv:lookup unfold:lookup_good_morphing.
+  }
+  8 : {
+    move => Γ A B i hA ihA ρ0 ρ1 Δ hρ hΔ.
+    rewrite /lookup_good_morphing => k A0.
+    elim /lookup_inv => h.
+    - move => > ? []*. subst.
+      rewrite /lookup_good_morphing in hρ.
+      move : h.
+      move /hρ.
+      asimpl.
+
+  }
+  - hauto l:on unfold:lookup_good_morphing db:wt.
+  - hauto q:on use:good_morphing_up db:wt.
+  - move => Γ A A' i B M M' hA ihA hB ihB hM ihM ρ0 ρ1 Δ hρ hΔ /=.
+    apply : WR_Lam; eauto with wt.
+    apply ihB. apply : good_morphing_up; auto.
+
+Lemma left_hand_reflexivity_mutual :
+  (forall Γ a b A, Γ ⊢ a ▻ b ∈ A -> Γ ⊢ a ▻ a ∈ A ) /\
+  (forall Γ a b A, Γ ⊢ a ▻+ b ∈ A -> Γ ⊢ a ▻ a ∈ A ) /\
+  (forall Γ, ⊢ Γ -> True).
+Proof.
+  apply wt_mutual_ind=>//; eauto with wt.
+  move => *. apply : WR_App.
+  sfirstorder.
+  best.
